hash out the invariants

networkInvariantPrototypes/toyLeaderElection/proof.dfy
@@ -9,12 +9,80 @@ module RingLeaderElectionProof {
   import opened DistributedSystem
   import opened Obligations
 
+  /***************************************************************************************
+  *                               Invariant and Definitons                               *
+  ***************************************************************************************/
+
+  // Message Invariant: self inductive
+  predicate ValidMessages(c: Constants, v: Variables) 
+    requires v.WF(c)
+  {
+    forall msg | msg in v.network.sentMsgs 
+    :: match msg 
+        case VoteReq(candidate) => c.ValidIdx(candidate)
+        case Vote(voter, candidate) => c.ValidIdx(voter) && c.ValidIdx(candidate)
+        case Leader(src) => c.ValidIdx(src)
+        case _ => true
+  }
+
+  // Message Invariant: self inductive
+  predicate LeaderMsgImpliesLocalQuorum(c: Constants, v: Variables) 
+    requires v.WF(c)
+    requires ValidMessages(c, v)
+  {
+    forall msg | msg in v.network.sentMsgs && msg.Leader?
+    :: SetIsQuorum(c.hostConstants[msg.src].clusterSize, v.hosts[msg.src].receivedVotes)
+  }
+
+  // Message Invariant: self inductive
+  predicate ReceivedVotesValidity(c: Constants, v: Variables) 
+    requires v.WF(c)
+  {
+    forall idx, voter | c.ValidIdx(idx) && voter in v.hosts[idx].receivedVotes 
+    :: Vote(voter, idx) in v.network.sentMsgs
+  }
+
+  // Message Invariant: self inductive
+  predicate VoteMsgImpliesVoterVoted(c: Constants, v: Variables)
+    requires v.WF(c)
+    requires ValidMessages(c, v)
+  {
+    forall msg | msg in v.network.sentMsgs && msg.Vote?
+    :: v.hosts[msg.voter].voted
+  }
+
+  predicate MessageInv(c: Constants, v: Variables) 
+  {
+    && v.WF(c)
+    && ValidMessages(c, v)
+    && LeaderMsgImpliesLocalQuorum(c, v)
+    && ReceivedVotesValidity(c, v)
+    && VoteMsgImpliesVoterVoted(c, v)
+  }
+
+  // Application Invariant
+  predicate VotersVoteOnce(c: Constants, v: Variables) 
+    requires v.WF(c)
+  {
+    forall m1, m2 |
+      && m1 in v.network.sentMsgs && m2 in v.network.sentMsgs
+      && m1.Vote? && m2.Vote?
+      && m1.voter == m2.voter
+    :: m1.candidate == m2.candidate
+  }
   
   predicate Inv(c: Constants, v: Variables)
   {
     && v.WF(c)
+    && MessageInv(c, v)
+    && VotersVoteOnce(c, v)
     && Safety(c, v)
   }
+
+
+  /***************************************************************************************
+  *                                        Proof                                         *
+  ***************************************************************************************/
 
   lemma InvImpliesSafety(c: Constants, v: Variables)
     requires Inv(c, v)
@@ -26,12 +94,28 @@ module RingLeaderElectionProof {
     ensures Inv(c, v)
   {}
 
+  lemma MessageInvInductive(c: Constants, v: Variables, v': Variables)
+    requires MessageInv(c, v)
+    requires Next(c, v, v')
+    ensures MessageInv(c, v')
+  {
+    assert MessageInv(c, v');  // dumb trigger
+  }
+
   lemma InvInductive(c: Constants, v: Variables, v': Variables)
     requires Inv(c, v)
     requires Next(c, v, v')
     ensures Inv(c, v')
   {
-    // TODO
+    assume false;
+    MessageInvInductive(c, v, v');
+    assert v.WF(c);
+    assert ValidMessages(c, v');
+    assert LeaderMsgImpliesLocalQuorum(c, v');
+    assert ReceivedVotesValidity(c, v');
+    assert VoteMsgImpliesVoterVoted(c, v');
+    assert VotersVoteOnce(c, v');
+    assert Safety(c, v');
   }
 }
 
